\documentclass{beamer}
\usepackage[utf8]{inputenc}
\usetheme{Madrid}
\usecolortheme{default}
\usepackage{amsmath,amssymb,amsfonts}
\usepackage{gvv}
\usepackage{txfonts}
\usepackage{tikz}
\usepackage{graphicx}

\title{2.10.34}
\author{EE25BTECH11013 - Bhargav}
\date{September 20, 2025}

\begin{document}
\frame{\titlepage}

\begin{frame}{Question}
Let $\vec{a} = \hat{i} - \hat{j}, \ \vec{b} = \hat{j} - \hat{k}, \ \vec{c} = \hat{k} - \hat{i}$.  
If $\vec{d}$ is a unit vector such that 
\[
\vec{a}^\top \vec{d} = 0 \quad \text{and} \quad 
\sbrak{\vec{b} \ \vec{c} \ \vec{d}} = 0,
\]
then $\vec{d}$ equals:
\[
\text{a) } \pm \frac{\hat{i}+\hat{j}-2\hat{k}}{\sqrt{6}} \quad
\text{b) } \pm \frac{\hat{i}+\hat{k}-\hat{j}}{\sqrt{3}} \quad
\text{c) } \pm \frac{\hat{i}+\hat{j}+\hat{k}}{\sqrt{3}} \quad
\text{d) } \pm \hat{k}
\]
\end{frame}

\begin{frame}{Vectors}
\[
\vec{a} = \myvec{1\\-1\\0}, \quad
\vec{b} = \myvec{0\\1\\-1}, \quad
\vec{c} = \myvec{-1\\0\\1}
\]
Let
\[
\vec{d} = \myvec{x\\y\\z}
\]
\end{frame}

\begin{frame}{Condition 1: Orthogonality}
\[
\vec{a}^\top \vec{d} = \myvec{1 & -1 & 0}\myvec{x\\y\\z} = x - y = 0
\]
\[
\Rightarrow x = y
\]
\end{frame}

\begin{frame}{Condition 2: Scalar Triple Product}
\[
\sbrak{\vec{b} \ \vec{c} \ \vec{d}} =
\det\myvec{0 & -1 & x \\ 1 & 0 & y \\ -1 & 1 & z} = 0
\]

Expanding:
\[
= (y+z) + x
\]
\[
\Rightarrow x + y + z = 0
\]
Since $x=y$,
\[
2x+z=0 \quad \Rightarrow \quad z=-2x
\]
\end{frame}

\begin{frame}{Unit Vector Condition}
\[
\vec{d} = \myvec{x\\x\\-2x}
\]
\[
\vec{d}^\top \vec{d} = x^2 + x^2 + (-2x)^2 = 6x^2 = 1
\]
\[
\Rightarrow x = \pm \frac{1}{\sqrt{6}}
\]
Thus,
\[
\vec{d} = \pm \frac{1}{\sqrt{6}} \myvec{1\\1\\-2}
\]
\end{frame}

\begin{frame}{Final Answer}
\[
\vec{d} = \pm \frac{\hat{i} + \hat{j} - 2\hat{k}}{\sqrt{6}}
\]
Correct option: **a**
\end{frame}

\end{document}

