\documentclass{beamer}
\usetheme{Madrid}

\usepackage{amsmath, amssymb, amsthm}
\usepackage{graphicx}
\usepackage{gensymb}
\usepackage[utf8]{inputenc}
\usepackage{hyperref}
\usepackage{tikz}
\usepackage{amsmath}

\title{5.12.7 Matgeo}
\author{AI25BTECH11012 - Garige Unnathi}
\date{}

\begin{document}

\frame{\titlepage}

% Question frame
\begin{frame}
\frametitle{Question}
 Solve the following equations for x and y :
 \begin{align*}
     (ax - by) + (a + 4b)= 0 \\
     (bx + ay) + (b - 4a)= 0
 \end{align*}
\end{frame}


% Solution steps
\begin{frame}
\frametitle{Solution}
given two equations :
 \begin{align}
     (ax - by) =  -(a + 4b) \\
     (bx + ay) = -(b - 4a)
 \end{align}

 these can be written as :

 \begin{align}
     \begin{bmatrix}a & -b \\ b & a\end{bmatrix}\begin{bmatrix}x \\ y\end{bmatrix} = \begin{bmatrix}-a-4b \\ 4a -b\end{bmatrix}
 \end{align}
\end{frame}

\begin{frame}
\frametitle{Solution}
\begin{align}
    \textbf{A}\textbf{X} = \textbf{B}
\end{align}
To find X we need to multiply $A^{-1}$ on both sides
\begin{align}
   X =A^{-1}B
\end{align}
\end{frame}

\begin{frame}
Finding $A^{-1}$ :
\begin{align}
    \begin{bmatrix}a-\lambda & -b \\ b & a-\lambda\end{bmatrix} = 0\\
    \lambda^{2} - 2a\lambda + a^{2} + b^{2} = 0
\end{align}
since :
\begin{align}
    \lvert \textbf{A}- \lambda\textbf{I} \rvert = 0\\
    \textbf{A}^{2} -2a\textbf{A} +(a^{2}+b^{2}) =0
\end{align}
Multiply both sides by \textbf{$A^{-1}$}:
\begin{align}
    \textbf{A} -2a\textbf{I}+\textbf{$A^{-1}$}(a^{2}+b^{2}) = 0\\
    \textbf{$A^{-1}$} = \frac{1}{a^{2}+b^{2}} (2a\textbf{I} - \textbf{A})\\
    \textbf{$A^{-1}$}= \begin{bmatrix}a & b \\ -b & a\end{bmatrix}
\end{align}
\end{frame}

 \begin{frame}
from the equation 0.5 :
\begin{align}
    \textbf{X} =\begin{bmatrix}a & b \\ -b & a\end{bmatrix}\begin{bmatrix}-a-4b  \\ 4a -b\end{bmatrix}
\end{align}
\begin{align}
   \textbf{X} =\begin{bmatrix}-a^{2} -b^{2} \\ 4a^{2} + 4b^{2}\end{bmatrix}
\end{align}
\end{frame}

 \begin{frame}
\frametitle{Solution}
Hence :
\begin{align*}
    x = -a^{2} -b^{2}\\
    y = 4a^{2} + 4b^{2}
\end{align*}

\end{frame}

\end{document}
